added generator for local bc address type

execution/theories/Generators.v
@@ -1,15 +1,25 @@
 Require Import ZArith Strings.Ascii Strings.String.
-From QuickChick Require Import QuickChick.
+From QuickChick Require Import QuickChick. Import QcNotation.
 From ExtLib.Structures Require Import Functor Applicative.
-
 
 From ConCert Require Import Blockchain.
 From ConCert Require Import LocalBlockchain.
 From ConCert Require Import Serializable.
 
-Print Amount.
+(* For monad notations *)
+Require Export ExtLib.Structures.Monads.
+Export MonadNotation. Open Scope monad_scope.
 
-Print Z.of_nat.
+From Coq Require Import List.
+Import ListNotations.
+
+(* Module DoNotation.
+Import ssrfun.
+Notation "'do!' X <- A ; B" :=
+  (bindGen A (fun X => B))
+  (at level 200, X ident, A at level 100, B at level 200).
+End DoNotation.
+Import DoNotation. *)
 
 (* Declare Instance genAmountSized : GenSized Amount.
 Declare Instance showAmount : Show Amount.
@@ -35,21 +45,42 @@ Instance shrinkAmount : Shrink Amount :=
 
 (* dummy implementation for now *)
 Definition empty_str : string := "".
+Definition sep : string := ", ".
 
+
+
+Record BaseGens {Setup Msg State : Type} := 
+  mkBaseGens {
+    (* Address          : Type; *)
+    genAddress       : G Blockchain.Address;
+    genSetup         : G Setup;
+    genMsg           : G Msg;
+    genState         : G State;
+    genSerializedVal : G SerializedValue;
+  }.
+
+
+Open Scope string_scope.
 Instance showChain (BaseTypes : ChainBase) : Show (@Chain BaseTypes) :=
   {|
-    show c := show (chain_height c)
+    show c := 
+      let height := show (chain_height c) in
+      let slot := show (current_slot c) in
+      let fin_height := show (finalized_height c) in
+        "{" ++ height ++ sep ++ slot ++ sep ++ fin_height ++ "}"
   |}.
 
-Print Chain.
+Close Scope string_scope.
 
 Instance genChainSized (BaseTypes : ChainBase) : GenSized (@Chain BaseTypes) :=
   {|
-    arbitrarySized n := returnGen (build_chain n n n (fun (a : Address) => Z.of_nat n))
+    arbitrarySized n := 
+      returnGen (build_chain n n n (fun (a : Blockchain.Address) => Z.of_nat n))
   |}.
 
-Print shrink.
-
+Definition a := vectorOf 2 (returnGen 10).
+Print a.
+Sample a.
 
 (* For now, shrinking does nothing *)
 Instance shrinkChain (BaseTypes : ChainBase) : Shrink (@Chain BaseTypes) :=
@@ -57,50 +88,95 @@ Instance shrinkChain (BaseTypes : ChainBase) : Shrink (@Chain BaseTypes) :=
     shrink c := cons c nil
   |}.
 
+Fixpoint mkMapFromList {B : Type}
+                       (address_eqb : Address -> Address -> bool)
+                       (genB : G B)
+                       (l : list Address) 
+                       : G (Address -> B) :=
+  match l with
+  | [] => b <- genB ;; returnGen (fun x => b)
+  | a::l' =>
+    b <- genB ;;
+    liftM 
+      (fun (mp : Address -> B) (x : Address) 
+        => if address_eqb x a then b else mp x) 
+      (mkMapFromList address_eqb genB l')
+  end.
+
+Definition mkMapFromListGen {B : Type}
+                          (address_eqb : Address -> Address -> bool)
+                          (genB : G B)
+                          (genListA : G (list Address)) 
+                          : G (Address -> B) :=
+  listA <- genListA ;; mkMapFromList address_eqb genB listA.
+
+
+
+Definition mkChainGen {Setup Msg State : Type}
+                        (baseGens : @BaseGens Setup Msg State) (BaseTypes : ChainBase)
+                        : nat -> G (@Chain BaseTypes)  := 
+  fun n =>
+  (* First construct context of Contract Addresses. *)
+  let g_address := genAddress baseGens in
+  let addr_eqb : Address -> Address -> bool := address_eqb in
+  let addr_list_gen : G (list Blockchain.Address) := vectorOf n g_address in
+    ch_height  <- arbitrarySized n ;;
+    cur_slot   <- arbitrarySized ch_height ;; (* We make sure current slot is <= chain height *)
+    mp         <- mkMapFromListGen addr_eqb (sized arbitrarySized) addr_list_gen ;; 
+    returnGen (build_chain ch_height cur_slot n (fun (a : Blockchain.Address) => Z.of_nat n)).
+
+
+
+Module LocalBlockchainGens.
+Require Import LocalBlockchain.
+Require Import BoundedN.
+
 Print LocalChainBase.
+
+Global Opaque Address. 
+
+Definition b10 : Address := BoundedN.of_Z_const AddrSize 10.
+Print N.to_nat.
+(* First we define an auxilliary generator for Addresses*)
+Definition genAddress : G (BoundedN.BoundedN AddrSize) :=
+  n <- arbitrarySized (N.to_nat AddrSize) ;;
+  let 
+    boundedNOpt : option (BoundedN.BoundedN AddrSize) := @BoundedN.of_nat AddrSize n
+  in returnGen match boundedNOpt with
+  | Some b => b
+  (* The None case should never happen since 'arbitrarySized' on AddrSize already ensures that
+     n <= AddrSized. *)
+  | None => BoundedN.of_Z_const AddrSize 0
+  end.
+
+
+
+End LocalBlockchainGens.
+
+
+
 Sample (@arbitrarySized Chain (genChainSized LocalChainBase) 2).
 
-Print genAmountSized.
-
-Definition a : Amount := 2.
 
 Sample (@arbitrarySized Amount genAmountSized 2).
 
-
-
-Print genZSized.
+Open Scope nat_scope.
 Definition n_is_zero_nat (n : nat) := n =? 0.
-QuickChick n_is_zero_nat.
-Print arbitrarySized.
+(* QuickChick n_is_zero_nat. *)
+
+
 (* Example of how to sample a specific type? *)
 Sample (@arbitrarySized Z genZSized 2).
-Print genAmountSized.
 Sample (@arbitrarySized Amount genZSized 2).
+(* How to go from arbitrarySized to arbitrary *)
+Print sized.
+Sample (@sized Z (@arbitrarySized Z genZSized)).
 
 
 Open Scope Z_scope.
 Definition n_is_zero (n : Z) := n =? 0.
-
-QuickChick n_is_zero.
-
-Print sized.
-Sample (@sized Z (@arbitrarySized Z genZSized)).
-
-(* 
-Instance sizedGenZ : GenSized Z :=
-  {|
-    arbitrarySized n := returnGen (Z.of_nat n)
-  |}.
-
-Print GenOfGenSized.
+(* QuickChick n_is_zero. *)
 
 
-Definition genZ := @GenOfGenSized Z sizedGenZ.
 
-(* Instance genZ : Gen Z :=
-  {|
-    arbitrary := returnGen Z0
-  |}. *) *)
 
-Check Amount.
-Derive  Arbitrary for Amount.
